clightplus_examples/xorlist/main0.v
@@ -1,12 +1,60 @@
-Require Import ITreelib.
-Require Import ModSem.
+Require Import CoqlibCCR.
 Require Import Skeleton.
+Require Import PCM.
+Require Import HoareDef.
+Require Import ProofMode.
+Require Import STB.
 Require Import Any.
-Require Import ClightPlusgen.
-Require Import main.
+Require Import ModSem.
+Require Import ModSemE.
+Require Import ClightPlusMem1.
+From compcert Require Export Ctypes Values AST Memdata Integers.
 
-(* TODO: one module embedding *)
-Definition _main : Errors.res Mod.t := compile prog "main".
+Set Implicit Arguments.
 
-Theorem valid_xor: exists xor, _xor = Errors.OK xor.
-Proof. eauto. Qed.
+Section SPEC.
+
+  Context `{@GRA.inG pointstoRA Σ}.
+  Context `{@GRA.inG allocatedRA Σ}.
+  Context `{@GRA.inG blocksizeRA Σ}.
+  Context `{@GRA.inG blockaddressRA Σ}.
+
+  Definition main_body : list val -> itree hEs val :=
+    fun _ => ;;;Ret (Vint (Int.repr 21)).
+
+  Definition main_spec : fspec :=
+    (mk_simple
+      (fun '() => (
+        (ord_top),
+        (fun varg => ⌜varg = (@nil val)↑⌝ ** Vnullptr (≃_m_null) Vnullptr),
+        (fun _ => ⌜True⌝)
+    )))%I.
+
+End SPEC.
+
+
+Section SMOD.
+
+  Context `{@GRA.inG pointstoRA Σ}.
+  Context `{@GRA.inG allocatedRA Σ}.
+  Context `{@GRA.inG blocksizeRA Σ}.
+  Context `{@GRA.inG blockaddressRA Σ}.
+
+  Definition mainSbtb: list (gname * fspecbody) :=
+    [("main", mk_specbody main_spec (cfunU main_body))].
+  
+  Definition SmainSem : SModSem.t := {|
+    SModSem.fnsems := mainSbtb;
+    SModSem.mn := "main";
+    SModSem.initial_mr := ε;
+    SModSem.initial_st := tt↑;
+  |}.
+
+  Definition Smain : SMod.t := {|
+    SMod.get_modsem := fun _ => SmainSem;
+    SMod.sk := Sk.unit;
+  |}.
+
+  Definition main stb : Mod.t := (SMod.to_tgt stb) Smain.
+
+End SMOD.
