clightplus_examples/xorlist/xorlist0.v
@@ -1,11 +1,38 @@
-Require Import ITreelib.
 Require Import ModSem.
 Require Import Skeleton.
-Require Import Any.
 Require Import ClightPlusgen.
 Require Import xorlist.
+Require Import main.
+From compcert Require Import Linking.
 
-Definition _xor : Errors.res Mod.t := compile prog "xorlist".
+Definition _xor : option Clight.program := link main.prog xorlist.prog.
 
-Theorem valid_xor: exists xor, _xor = Errors.OK xor.
-Proof. eauto. Qed.
+Definition xor : Errors.res Mod.t := 
+    match _xor with
+    | Some xor => compile xor "xorlist"
+    | None => Errors.Error [Errors.MSG "no link"]
+    end.
+
+Definition _msk : Errors.res Sk.t :=
+    match _xor with
+    | Some xor => mem_skel xor
+    | None => Errors.Error [Errors.MSG "no link"]
+    end.
+
+Theorem msk_xor: exists msk, _msk = Errors.OK msk.
+Proof. 
+  unfold _msk, _xor. 
+  eassert (link prog xorlist.prog = _).
+  { vm_compute (link _ _). eauto. }
+  rewrite H. clear H. destruct Ctypes.link_build_composite_env. destruct a.
+  vm_compute (mem_skel _). eauto.
+Qed.
+
+Theorem valid_xor: exists p, xor = Errors.OK p.
+Proof.
+  unfold xor, _xor.
+  eassert (link prog xorlist.prog = _).
+  { vm_compute (link _ _). eauto. }
+  rewrite H. clear H. destruct Ctypes.link_build_composite_env. destruct a. eauto.
+Qed.
+
