clightplus_examples/xorlist/xorlistall.v
@@ -1,0 +1,36 @@
+
+  Section SIMFUNS.
+  Variable xorlink : Clight.program.
+  Variable xormod : Mod.t.
+  Hypothesis VALID_link : xorlist0._xor = Some xorlink.
+  Hypothesis VALID_comp : compile xorlink "xorlist" = Errors.OK xormod.
+  Let mfsk : Sk.t := [("malloc", Gfun (F:=Clight.fundef) (V:=type) (Ctypes.External EF_malloc (Tcons tulong Tnil) (tptr tvoid) cc_default)); ("free", Gfun (Ctypes.External EF_free (Tcons (tptr tvoid) Tnil) tvoid cc_default))].
+  (* Require Import ClightPlusMem01Proof. *)
+
+  Variable xor0 : Mod.t.
+  Hypothesis VALID : xorlist0._xor = Errors.OK xor0.
+
+  Theorem correct : refines2 [xormod; ClightPlusMem0.Mem mfsk] [xorlist1.xor xormod GlobalStb; main GlobalStb; ClightPlusMem1.Mem mfsk].
+  Proof.
+    eapply adequacy_local_strong_l. econs; cycle 1.
+    { econs; [ss|]. econs; ss. }
+    i. econs; cycle 1.
+    { econs; [|ss]. apply correct_mod; et. inv SKINCL. inv H6. ss. }
+    unfold _xor, compile, get_sk in VALID.
+    destruct Pos.eq_dec; [|clarify].
+    destruct Coqlib.list_norepet_dec; ss. des_ifs_safe.
+    econstructor 1 with (wf := wf) (le := top2); et; ss; cycle 1.
+    { eexists. econs. apply to_semantic. iIntros. et. }
+    (* each functions has simulation relation *)
+    econs; cycle 1.
+    econs; cycle 1.
+    econs; cycle 1.
+    econs; cycle 1.
+    econs; et.
+    all: des_ifs; inv SKINCL; inv H6; ss.
+    - eapply sim_delete_tl; et.
+    - eapply sim_delete_hd; et.
+    - eapply sim_add_tl; et.
+    - eapply sim_add_hd; et.
+    Unshelve. exact tt.
+  Qed.
